\documentclass[12pt]{article}
\usepackage{graphicx}
\usepackage{graphics}
\usepackage{refstyle}
\usepackage{amsmath}
\usepackage{caption}
\usepackage{float}
\usepackage{booktabs}
\usepackage{array}
\usepackage{amssymb}
\usepackage{booktabs}
\renewcommand{\vec}{\boldsymbol}
\graphicspath{{/storage/self/primary/Download/latexnew/fig}}                                             
\graphicspath{{/storage/self/primary/Download/latexnew/table}}


\begin{document}
\title{\textbf{VECTOR}}
\date{}
\maketitle
\textbf{Question:} $\vec{P}$ and $\vec{Q}$ are any two points lying on the sides $DC$ and $AD$ respectively of a parallelogram $ABCD$.Show that, $ar(\triangle APB)=ar(\triangle BQC)$.


\textbf{Figure:}
\begin{figure}[H]
    \centering
    \includegraphics[width=\columnwidth]{fig/1.png}
    \caption{}
    \label{fig:fig:1}
\end{figure}


\textbf{Solution:}\\
Using formulas: \begin{enumerate}
\item Area of a parallelogram with sides $\vec{a}$ and $\Vec{b}$ is = $\frac{1}{2}\big|\Vec{a}\times\Vec{b}\big|$ square units = $\frac{1}{2}\big|a.b\sin{\theta}\big|$
 \item Area of a triangle with vertices $(x_1,y_1),(x_2,y_2),(x_3,y_3)$ is =  $\frac{1}{2}\times$
  \begin{tabular}{|c c c|}
     1&1&1\\
     $x_1$&$x_2$&$x_3$\\
     $y_1$&$y_2$&$y_3$\\
  \end{tabular} square units . (only positive values will be taken as negative value of area is not possible)

\item If a triangle and a parallelogram are on the same base and between the same parallels, then area of the triangle is equal to half the area of the parallelogram.

\end{enumerate}
From \figref{fig:1} ,
considering $\triangle BQC$ and parallelogram $ ABCD$, having \underline{same base $BC$} and, \underline{$AD$ is parallel to $BC$}.\\

\begin{equation}
\implies \triangle BQC = \frac{1}{2}\times ar ABCD.
  \label{eq:eq:1}
\end{equation}

Considering $\triangle APB$ and parallelogram $ABCD$ , having \underline{same base $AB$} and,\underline{$DC$ is parallel to $AB$}.

\begin{equation}
\implies \triangle APB = \frac{1}{2}\times ar ABCD.
	\label{eq:eq:2}
\end{equation}

By comparing \eqref{eq:1} and \eqref{eq:2} we obtain that,

\begin{equation}
    ar(\triangle APB) =  ar(\triangle BQC).
\end{equation}
\begin{center}
 Hence proved.

\end{center}

\textbf{Proof by the help of diagram :}(\figref{fig:1},\tabref{tab:1},\tabref{tab:2})\\
Let the points $\vec{Q}$ and $\Vec{P}$ divide $AD$ and $CD$ by $k_1:1$ and $k_2:1$ ratio respectively.
\begin{table}[H]
   \centering
   \input{table/tab1.tex}
   \caption{Table of input parameters}
   \label{tab:tab:1}
\end{table}




\begin{table}[H]
    \centering                                       
    \input{table/tab2.tex}                          
    \caption{Table of output parameters}
    \label{tab:tab:2}
 \end{table}


For the $\triangle BQC$, the vertices of the triangle are
 
   $\Vec{B}=\begin{pmatrix}
       6\\0
   \end{pmatrix},
   \Vec{Q}=\begin{pmatrix}
       \frac{2k_1}{k_1+1}\\\frac{5k_1}{k_1+1}
   \end{pmatrix},
   \Vec{C}=\begin{pmatrix}
       8\\5
   \end{pmatrix}$

   
$\implies \triangle BQC =
\begin{tabular}{|c c c|}
       1 &1&1\\
       6&$\frac{2k_1}{k_1+1}$&8 \\
       0&$\frac{5k_1}{k_1+1}$&5
   \end{tabular}\\
\frac{1}{2} \times \big|1(\frac{2k_1}{k_1+1}.5-\frac{5k_1}{k_1+1}.8)-6(5.1-\frac{5k_1}{k_1+1}.1)+0\big|\\
 = \frac{1}{2} \times\big |\frac{-40k_1+10k_1-30}{k_1+1}\big|\\
 =\frac{1}{2} \times30\\
 =15 $ square units.


For the $\triangle APB$, the vertices of the triangle are

   $\Vec{A}=\begin{pmatrix}
       0\\0
   \end{pmatrix},
   \Vec{P}=\begin{pmatrix}
       \frac{8k_2+2}{k_2+1}\\5
   \end{pmatrix},
   \Vec{B}=\begin{pmatrix}
       6\\0
   \end{pmatrix}$\\
   $\implies \triangle APB =
   \begin{tabular}{|c c c|}
       1 &1&1\\
       0&$\frac{8k_2+2}{k_2+1}$&6 \\
       0&5&0
   \end{tabular}\\
 = \frac{1}{2} \times \big |1(\frac{8k_2+2}{k_2+1}.0-6.5)+0+0\big|\\
 = \frac{1}{2} \times\big |-30\big|\\
 =\frac{1}{2} \times30\\
 =15 $ square units.


 
  For parallelogram $ABCD$,the vertices are

   $\Vec{A}=\begin{pmatrix}
       0\\0
   \end{pmatrix},
 \Vec{B}=\begin{pmatrix}
       6\\0
   \end{pmatrix},
   \Vec{C}=\begin{pmatrix}
       8\\5
   \end{pmatrix},
   \Vec{D}=\begin{pmatrix}
       2\\5
   \end{pmatrix}$
   
$\implies ar ABCD = a.b.\sin \theta$\\
 =$6.\sqrt{29}.\sin(\sin^{-1}{\frac{5}{\sqrt{29}}})$\\
=$6.\sqrt{29}.\frac{5}{\sqrt{29}}$\\
=30 square units.


 Therefore,$ar ABCD = \frac{1}{2}\times ar \triangle APB = \frac{1}{2}\times ar \triangle BQC$(proved).


\end{document}

