\documentclass[12pt]{article}
\usepackage{graphicx}
\usepackage{graphics}
\usepackage{refstyle}
\usepackage{amsmath}
\usepackage{caption}
\usepackage{float}
\usepackage{booktabs}
\usepackage{array}
\usepackage{amssymb}
\usepackage{booktabs}
\let\vec\mathbf
\providecommand{\brak}[1]{\ensuremath{\left(#1\right)}}
\graphicspath{{/storage/self/primary/Download/latexnew/fig}}                                            
\graphicspath{{/storage/self/primary/Download/latexnew/table}}
\begin{document}
\title{\textbf{VECTOR}}
\date{}
\maketitle
\textbf{Question:} $\vec{P}$ and $\vec{Q}$ are any two points lying on the sides $DC$ and $AD$ respectively of a parallelogram $ABCD$.Show that, $ar\brak{\triangle APB}=ar\brak{\triangle BQC}$.


\textbf{Figure:}
\begin{figure}[H]
    \centering
   \includegraphics[width=\columnwidth]{fig/1.png}
    \caption{}
    \label{fig:fig:1}
\end{figure}


\textbf{Solution:}
From \figref{fig:1} ,
considering $\triangle BQC$ and parallelogram $ ABCD$, having \underline{same base $BC$} and, \underline{$AD$ is parallel to $BC$}.\\
\begin{align}
\implies \triangle BQC = \frac{1}{2}\times ar ABCD.
  \label{eq:eq:1}
\end{align}
Considering $\triangle APB$ and parallelogram $ABCD$ , having \underline{same base $AB$} and,\underline{$DC$ is parallel to $AB$}.

\begin{align}
\implies \triangle APB = \frac{1}{2}\times ar ABCD.
\label{eq:eq:2}
\end{align}

By comparing \eqref{eq:1} and \eqref{eq:2} we obtain that,

\begin{align}
    ar\brak{\triangle APB} =  ar\brak{\triangle BQC}.
\end{align}
\begin{center}
 Hence proved.

\end{center}

\textbf{Proof by the help of diagram :}\brak{\figref{fig:1},\tabref{tab:1},\tabref{tab:2}}\\
Let the points $\vec{Q}$ and $\Vec{P}$ divide $AD$ and $CD$ by $k_1:1$ and $k_2:1$ ratio respectively.
\begin{table}[H]
   \centering
   \input{table/tab1.tex}
   \caption{Table of input parameters}
   \label{tab:tab:1}
\end{table}




\begin{table}[H]
    \centering                                      
    \input{table/tab2.tex}                          
    \caption{Table of output parameters}
	\label{tab:tab:2}
 \end{table}


For the $\triangle BQC$, the vertices of the triangle are taken from \tabref{tab:1} and \tabref{tab:2}.

\begin{align}
\implies\triangle BQC=
\frac{1}{2}\begin{tabular}{|c c c|}
       1 &1&1\\
       6&$\frac{2k_1}{k_1+1}$&8 \\
       0&$\frac{5k_1}{k_1+1}$&5
   \end{tabular}\\
   \xrightarrow{C_2'=C_2-C_1,C_3'=C_3-C_1}\frac{1}{2} \begin{tabular}{|c c c|}
       1 &0&0\\
       6&$\frac{-4k_1-6}{k_1+1}$&2 \\
       0&$\frac{5k_1}{k_1+1}$&5
   \end{tabular}\\
 =\frac{1}{2} \times30\\
 =15 \end{align}


For the $\triangle APB$, the vertices of the triangle are taken from \tabref{tab:1} and \tabref{tab:2}.
   \begin{align}
	   \implies \triangle APB =\frac{1}{2}
   \begin{tabular}{|c c c|}
       1 &1&1\\
       0&$\frac{8k_2+2}{k_2+1}$&6 \\
       0&5&0
   \end{tabular}\\
 =\frac{1}{2} \times30\\
 =15 \end{align}


 
  For parallelogram $ABCD$,the vertices are taken from \tabref{tab:1} nd \tabref{tab:2}.
\begin{align}   
\implies ar ABCD = ab\sin\theta\\
 =6\sqrt{29}\sin\brak{\sin^{-1}{\frac{5}{\sqrt{29}}}}\\
=6\sqrt{29}\frac{5}{\sqrt{29}}\\
=30\end{align}


 Therefore,$ar ABCD = 2\times ar\triangle APB = 2\times ar \triangle BQC$\brak{proved}.\\
 


\end{document}

